proofs/proofsystem/ProofSystem.v
@@ -1,0 +1,335 @@
+(*Here, for the core logic (no definitions/inductive types),
+  we define equivalences in terms of Coq operations*)
+Require Import FullInterp.
+Require Import Alpha.
+Set Bullet Behavior "Strict Subproofs".
+
+(*We work at the level of satisfying interpretations, since
+  we need to quantify over valuations. If we fix valuations,
+  some of this (like the quantifier equivalence) does not
+  hold*)
+
+(*Quantifiers*)
+
+Lemma tforall_rewrite_ty {gamma} {f: formula} {x: vsymbol} 
+  (Hty: formula_typed gamma (Fquant Tforall x f))
+  (y: string):
+  formula_typed gamma (safe_sub_f (Tvar (y, snd x)) x f).
+Proof.
+  destruct x; simpl in *.
+  inversion Hty; subst.
+  apply safe_sub_f_typed; auto.
+  constructor. auto.
+Qed.
+
+Lemma tforall_rewrite {gamma: context} {gamma_valid: valid_context gamma}
+  {pd: pi_dom} {pf: pi_funpred gamma_valid pd}
+  {Hfull: full_interp gamma_valid pd pf}
+  {x: vsymbol}
+  {f: formula} {Hty: formula_typed gamma (Fquant Tforall x f)}:
+  satisfies gamma_valid pd pf Hfull (Fquant Tforall x f) Hty <->
+  (forall (y: string), satisfies gamma_valid pd pf Hfull
+    (safe_sub_f (Tvar (y, snd x)) x f) (tforall_rewrite_ty Hty y)).
+Proof.
+  unfold satisfies. destruct x as [xn xt]; subst; simpl in *. 
+  split; intros; simpl_rep_full.
+  - (*easy direction*)
+    specialize (H vt vv). revert H; simpl_rep_full;
+    rewrite simpl_all_dec; intros.
+    erewrite safe_sub_f_rep. apply H.
+    Unshelve. inversion Hty; subst; constructor; auto.
+  - (*Harder - why this is NOT true if we fix valuation -
+      we need to choose a valuation that sends y to d*)
+    rewrite simpl_all_dec.
+    intros d.
+    specialize (H xn vt (substi pd vt vv (xn, xt) d)).
+    generalize dependent (tforall_rewrite_ty Hty xn).
+    simpl. unfold safe_sub_f.
+
+    destruct (in_bool vsymbol_eq_dec (xn, xt) (fmla_fv f)).
+    destruct ( existsb (fun x : vsymbol => in_bool vsymbol_eq_dec x (fmla_bnd f))
+    (tm_fv (Tvar (xn, xt)))).
+    + rewrite <- sub_var_f_equiv, sub_var_f_eq; intros.
+      erewrite fmla_rep_irrel in H.
+      erewrite <- a_convert_f_rep in H.
+      apply H.
+    + rewrite <- sub_var_f_equiv, sub_var_f_eq; intros.
+      erewrite fmla_rep_irrel. apply H.
+    + intros. erewrite fmla_rep_irrel. apply H.
+Qed.
+
+(*Alternate approach: natural deduction*)
+
+(*The other method does not work, since it implicitly involves
+  proving (essentially) both soundness and completeness.
+  Completeness is hard, we do not show it. We only
+  prove soundness*)
+Require Import Task.
+(*Reserved Notation "g ; d '|--' f" (at level 90).*)
+
+(*All of the sound transformations can be derived*)
+Inductive derives {gamma: context}: task gamma -> Prop :=
+  | D_trans: forall (tr: trans gamma) (t: task gamma) 
+    (l: list (task gamma)),
+    task_wf t ->
+    sound_trans tr ->
+    tr t = l ->
+    (forall x, In x l -> derives x) ->
+    derives t.
+
+(*Soundness is trivial*)
+Theorem soundness {gamma: context} (t: task gamma):
+  derives t ->
+  task_valid t.
+Proof.
+  intros Hd.
+  induction Hd. subst.
+  apply (H0 _ H). subst; auto.
+Qed.
+
+(*Now we give some of the familiar proof rules, as transformations.
+  Some of them we may change to the why3 versions*)
+
+Section NatDed.
+
+Context {gamma: context}.
+
+(*Axiom rule*)
+Definition axiom_trans (t: task gamma) : list (task gamma) :=
+  if in_bool formula_eq_dec (task_goal t) (task_delta t)
+  then nil else [t].
+
+Lemma axiom_trans_sound : sound_trans axiom_trans.
+Proof.
+  unfold sound_trans, axiom_trans. intros.
+  destruct (in_bool_spec formula_eq_dec (task_goal t) (task_delta t)).
+  - unfold task_valid.
+    split; auto. intros. unfold log_conseq.
+    intros. unfold satisfies in *. intros.
+    specialize (H0 _ i vt vv). 
+    erewrite fmla_rep_irrel. apply H0.
+  - simpl in H. apply H; auto.
+Qed.
+
+(*And now the deduction rule*)
+Theorem D_axiom (t: task gamma) :
+  task_wf t ->
+  In (task_goal t) (task_delta t) ->
+  derives t.
+Proof.
+  intros. eapply (D_trans axiom_trans). auto.
+  apply axiom_trans_sound. 
+  unfold axiom_trans.
+  reflexivity. intros.
+  destruct (in_bool_spec formula_eq_dec (task_goal t) (task_delta t));
+  auto; try contradiction.
+Qed.
+
+(*And*)
+(*TODO: move*)
+(*TODO: maybe get rid of vars in task*)
+Definition task_change_goal (t: task gamma) (goal: formula) : task gamma :=
+  mk_task gamma (task_delta t) goal.
+
+Definition andI_trans : trans gamma :=
+  fun t =>
+  match (task_goal t) with
+  | Fbinop Tand f1 f2 => [task_change_goal t f1; task_change_goal t f2]
+  | _ => [t]
+  end.
+
+Lemma andT_trans_sound: sound_trans andI_trans.
+Proof.
+  unfold sound_trans, andI_trans. intros.
+  destruct (task_goal t) eqn : Ht; simpl in H; try solve[apply H; auto].
+  destruct b; simpl in H; try solve[apply H; auto].
+  unfold task_valid. split; auto.
+  intros.
+  unfold log_conseq, satisfies. intros.
+  generalize dependent (task_goal_typed w_wf).
+  rewrite Ht; intros. simpl_rep_full.
+  bool_to_prop.
+  split.
+  - specialize (H (task_change_goal t f1) (ltac:(auto))).
+    unfold task_valid, task_change_goal in H; simpl in H.
+    destruct H. specialize (H1 gamma_valid H).
+    unfold log_conseq, satisfies in H1.
+    erewrite fmla_rep_irrel. apply H1; auto.
+    intros. erewrite fmla_rep_irrel. apply H0.
+    Unshelve. auto.
+  - specialize (H (task_change_goal t f2) (ltac:(auto))).
+    unfold task_valid, task_change_goal in H; simpl in H.
+    destruct H. specialize (H1 gamma_valid H).
+    unfold log_conseq, satisfies in H1.
+    erewrite fmla_rep_irrel. apply H1; auto.
+    intros. erewrite fmla_rep_irrel. apply H0.
+    Unshelve. auto.
+Qed.
+
+(*And now the deduction rule*)
+Theorem D_andI (delta: list formula)
+  (f1 f2: formula):
+  task_wf (delta, (Fbinop Tand f1 f2)) ->
+  derives (delta, f1) ->
+  derives (delta, f2) ->
+  derives (delta, Fbinop Tand f1 f2).
+  task_wf (mk_tasn delta vars ())
+
+Theorem D_axiom (t: task gamma) :
+  task_wf t ->
+  In (task_goal t) (task_delta t) ->
+  derives t.
+Proof.
+  intros. eapply (D_trans axiom_trans). auto.
+  apply axiom_trans_sound. 
+  unfold axiom_trans.
+  reflexivity. intros.
+  destruct (in_bool_spec formula_eq_dec (task_goal t) (task_delta t));
+  auto; try contradiction.
+Qed.
+
+
+    
+  
+  split; [apply H |].
+  apply /andP.
+
+  
+  
+  constructor.
+
+
+
+
+intros. apply H2; subst; auto.
+
+
+  subst.
+
+
+
+  | D_axiom : forall delta f,
+    In f delta ->
+    gamma ; delta |-- f
+    (*TODO: see if we need weakening, perm*)
+    (*
+  | derives_weakening: forall fs f g,
+    derives fs f ->
+    derives (g :: fs) f
+  | derives_perm: forall fs1 fs2 f,
+    Permutation fs1 fs2 ->
+    derives fs1 f ->
+    derives fs2 f*)
+  (*and*)
+  | D_andI: forall delta f g,
+    gamma; delta |-- f ->
+    gamma; delta |-- g ->
+    (*TODO: notations for these*)
+    gamma; delta |-- (Fbinop Tand f g)
+  | D_andE1: forall delta f g,
+    gamma; delta |-- Fbinop Tand f g ->
+    gamma; delta |-- f
+  | D_andE2: forall delta f g,
+    gamma; delta |-- Fbinop Tand f g ->
+    gamma; delta |-- g
+  (*or*)
+  | D_orI1: forall delta f g,
+    gamma; delta |-- f ->
+    gamma; delta |-- Fbinop Tor f g
+  | D_orI2: forall delta f g,
+    gamma; delta |-- g ->
+    gamma; delta |-- Fbinop Tor f g
+  | D_orE: forall delta f g c,
+    gamma; delta |-- Fbinop Tor f g ->
+    gamma; f:: delta |-- c ->
+    gamma; f:: delta |-- c ->
+    gamma; delta |-- c
+  (*true*)
+  | D_trueI: forall delta,
+    gamma; delta |-- Ftrue
+  (*false*)
+  | D_falseE: forall delta f,
+    gamma; delta |-- Ffalse ->
+    gamma; delta |-- f
+  (*negation - as A -> False*)
+  (*
+  | D_notI: forall gamma f,
+    f :: gamma |-- Ffalse ->
+    gamma |-- Fnot f
+  | D_notE: forall gamma f,
+    gamma |-- Fnot f ->
+    gamma |-- f ->
+    gamma |-- Ffalse*)
+  (*implication*)
+  | D_implI: forall delta f g,
+    gamma; f :: delta |-- g ->
+    gamma; delta |-- Fbinop Timplies f g
+  | D_implE: forall delta f g,
+    gamma; delta |-- Fbinop Timplies f g ->
+    gamma; delta |-- f ->
+    gamma; delta |-- g
+  (*quantifiers*)
+  | D_allI: forall delta x f a,
+    ~ In a (map fst (fmla_fv f)) ->
+    (* gamma |- f[a/x] proves gamma |- forall x, f
+      if a not free in f*)
+    gamma; delta |-- safe_sub_f (Tvar (a, snd x)) x f ->
+    gamma; delta |-- Fquant Tforall x f
+  | D_allE: forall delta x f t,
+    gamma; delta |-- Fquant Tforall x f ->
+    gamma; delta |-- safe_sub_f t x f
+  | D_exI: forall delta x f t,
+    gamma; delta |-- safe_sub_f t x f ->
+    gamma; delta |-- Fquant Texists x f
+  | D_exE: forall delta x f a c,
+    gamma; delta |-- Fquant Texists x f ->
+    gamma; safe_sub_f (Tvar (a, snd x)) x f :: delta |-- c ->
+    ~ In a (map fst (fmla_fv f)) ->
+    gamma; delta |-- c
+  (*TODO: will likely remove all of the above later*)
+  (*We can derive any sound transformation*)
+  | D_trans: forall delta vars f
+    (tr: trans gamma),
+    sound_trans
+where "g ; d '|--' f" := (derives g d f).
+
+
+(*Implication*)
+Lemma fimpl_rewrite_ty1 {gamma} {f1 f2: formula}
+(Hty: formula_typed gamma (Fbinop Timplies f1 f2)):
+formula_typed gamma f1.
+Proof.
+  Search formula_typed Fbinop.
+  inversion Hty; subst; auto.
+Qed.
+
+Lemma fimpl_rewrite {gamma: context} {gamma_valid: valid_context gamma}
+{pd: pi_dom} {pf: pi_funpred gamma_valid pd}
+{Hfull: full_interp gamma_valid pd pf}
+{f1 f2: formula} {Hty: formula_typed gamma (Fbinop Timplies f1 f2)}:
+satisfies gamma_valid pd pf Hfull (Fbinop Timplies f1 f2) Hty <->
+(satisfies gamma_valid pd pf Hfull f1 (proj1' (typed_binop_inv Hty)) ->
+satisfies gamma_valid pd pf Hfull f2 (proj2' (typed_binop_inv Hty))).
+Proof.
+  unfold satisfies. split; intros.
+  - specialize (H vt vv).
+    revert H; simpl_rep_full. rewrite bool_of_binop_impl, simpl_all_dec.
+    auto.
+  - simpl_rep_full. rewrite bool_of_binop_impl, simpl_all_dec. intros.
+    apply H. 
+    intros.
+    
+    Search implb is_true.
+.
+
+
+Lemma tforall_rewrite {gamma: context} {gamma_valid: valid_context gamma}
+  {pd: pi_dom} {pf: pi_funpred gamma_valid pd}
+  {Hfull: full_interp gamma_valid pd pf}
+  {x: vsymbol}
+  {f: formula} {Hty: formula_typed gamma (Fquant Tforall x f)}:
+  satisfies gamma_valid pd pf Hfull (Fquant Tforall x f) Hty <->
+  (forall (y: string), satisfies gamma_valid pd pf Hfull
+    (safe_sub_f (Tvar (y, snd x)) x f) (tforall_rewrite_ty Hty y)).
+
+  
